CoqBB5/Deciders_CustomParameters/Decider_RepWL_CustomParameters.v
@@ -2,7 +2,7 @@ Require Import List.
 
 From CoqBB5 Require Import BB52Statement.
 From CoqBB5 Require Import TM.
-From CoqBB5 Require Import Decider_Pipeline.
+From CoqBB5 Require Import BB52Decider_Pipeline.
 
 Definition tm_RWL:list ((TM Σ)*(DeciderType)) :=
 (makeTM BR0 HR1 AL1 CL0 DR1 CL1 CL1 ER0 BL1 ER1,RWL 2 3)::
