CoqBB5/Deciders_CustomParameters/Decider_Verifier_FAR_CustomParameters.v
@@ -2,7 +2,7 @@ Require Import List.
 
 From CoqBB5 Require Import BB52Statement.
 From CoqBB5 Require Import TM.
-From CoqBB5 Require Import Decider_Pipeline.
+From CoqBB5 Require Import BB52Decider_Pipeline.
 
 Definition DFA_from_list(ls:list(nat*nat))(x:nat)(i:Σ) :=
   let (a,b) := nth x ls (0,0) in
